src/interactive/FStarC.Interactive.Incremental.fst
@@ -18,6 +18,7 @@ module FStarC.Interactive.Incremental
 open FStarC.Effect
 open FStarC.List
 open FStarC
+open FStarC.Class.Show
 open FStarC.Range
 open FStarC.Getopt
 open FStarC.Ident
@@ -145,12 +146,14 @@ let push_decls (push_kind:push_kind)
   : qst (list query)
   = let! qs = map (push_decl push_kind with_symbols write_full_buffer_fragment_progress) ds in
     return (List.flatten qs)
-  
+
+let repl_task_of_entry (_, (p, _)) = p
+
 let pop_entries (e:list repl_stack_entry_t)
   : qst (list query)
   = map (fun _ -> as_query Pop) e
   
-let repl_task (_, (p, _)) = p
+// let repl_task (_, (p, _)) = p
 
 let push_kind_geq pk1 pk2 =
   pk1=pk2 || (
@@ -159,16 +162,45 @@ let push_kind_geq pk1 pk2 =
   | LaxCheck, SyntaxCheck -> true
   | _ -> false
   )
+
+
+let scan_query_deps st (queries:list query) =
+  let to_scan =
+    List.filter_map
+      (fun q ->
+        match q.qq with
+        | Push { push_code_or_decl = Inr (d, _) } -> Some d
+        | _ -> None)
+      queries
+  in            
+  let deps = FStarC.Syntax.DsEnv.dep_graph st.repl_env.dsenv in
+  let deps = FStarC.Parser.Dep.copy_deps deps in
+  let env = { st.repl_env with dsenv=FStarC.Syntax.DsEnv.set_dep_graph st.repl_env.dsenv deps } in
+  let filenames_to_load =
+    FStarC.Parser.Dep.collect_deps_of_decl
+      deps
+      st.repl_fname
+      to_scan
+      FStarC.CheckedFiles.load_parsing_data_from_cache
+  in
+
+  let tasks = List.rev <| List.map mk_ld_single filenames_to_load in
+  Format.print1 "Initial files loaded: %s\n" (show <| FStarC.Parser.Dep.all_files deps);
+  Format.print1 "Decls scanned: %s\n" (show to_scan);
+  Format.print1 "Additional files to load: %s\n" (show filenames_to_load);
+  tasks, {st with repl_env=env}
+      
 (* Find a prefix of the repl stack that matche a prefix of the decls ds, 
    pop the rest of the stack
    and push the remaining suffix of decls
 *)
-let inspect_repl_stack (s:repl_stack_t)
+let inspect_repl_stack (s:repl_stack_t) (st:repl_state)
                        (ds:list (decl & code_fragment))
                        (push_kind : push_kind)
+                       (scan_deps:bool)
                        (with_symbols:bool)
                        (write_full_buffer_fragment_progress: fragment_progress -> unit)                       
-  : qst (list query & list json)
+  : qst (list query & list json & repl_state)
   = let entries = List.rev s in
     let push_decls = push_decls push_kind with_symbols write_full_buffer_fragment_progress in
     match BU.prefix_until 
@@ -177,11 +209,10 @@ let inspect_repl_stack (s:repl_stack_t)
     with
     | None ->
       let! ds = push_decls ds in
-      return (ds, [])
+      return (ds, [], st)
     
-    | Some (prefix, first_push, rest) ->
+    | Some (_prefix, first_push, rest) ->
       let entries = first_push :: rest in
-      let repl_task (_, (p, _)) = p in
       let rec matching_prefix (accum:list json) (lookups:list query) entries (ds:list (decl & code_fragment))
         : qst (list query & list json)
         = match entries, ds with
@@ -189,14 +220,14 @@ let inspect_repl_stack (s:repl_stack_t)
             return (lookups, accum)
             
           | e::entries, d::ds -> (
-            match repl_task e with
+            match repl_task_of_entry e with
             | Noop -> 
               matching_prefix accum lookups entries (d::ds)
-            | PushFragment (Inl frag, _, _) ->
+            | PushFragment (Inl frag, _, _, _) ->
               let! pops = pop_entries (e::entries) in
               let! pushes = push_decls (d::ds) in
               return (lookups @ pops @ pushes, accum)
-            | PushFragment (Inr d', pk, issues) ->
+            | PushFragment (Inr d', pk, issues, _) -> (
               if eq_decl (fst d) d' && pk `push_kind_geq` push_kind
               then (
                 let d, s = d in
@@ -211,6 +242,9 @@ let inspect_repl_stack (s:repl_stack_t)
                    let! pushes = push_decls (d::ds) in
                    return (pops @ lookups @ pushes, accum)
             )
+            // | LDSingle _ -> 
+
+            )
 
          | [], ds ->
            let! pushes = push_decls ds in
@@ -220,7 +254,8 @@ let inspect_repl_stack (s:repl_stack_t)
            let! pops = pop_entries es in
            return (lookups@pops, accum)
       in
-      matching_prefix [] [] entries ds 
+      let! queries, json = matching_prefix [] [] entries ds in
+      return (queries, json, st)
 
 (* A reload_deps request just pops away the entire stack of PushFragments.
    We also push on just the `module A` declaration after popping. That's done below. *)
@@ -228,7 +263,7 @@ let reload_deps repl_stack =
   let pop_until_deps entries
   : qst (list query)
   = match BU.prefix_until
-            (fun e -> match repl_task e with
+            (fun e -> match repl_task_of_entry e with
                       | PushFragment _ | Noop -> false
                       | _ -> true)
             entries
@@ -268,11 +303,17 @@ let run_full_buffer (st:repl_state)
                     (request_type:full_buffer_request_kind)
                     (with_symbols:bool)
                     (write_full_buffer_fragment_progress: fragment_progress -> unit)
-  : list query & list json
+  : list query & list json & repl_state
   = // updating the vfs entry allows dependence scanning on the file to
     // to use the latest snapshot of the file, rather than what was present
     // in the buffer when the IDE was started. This is especially useful when
     // creating a new file and launching F* on it
+    if Debug.any() then (
+      Format.print1 "run_full_buffer: repl_state=%s\n"
+          (show st);
+      Format.print1 "run_full_buffer: repl_stack=%s\n"
+          (show (!repl_stack))
+    );
     FStarC.Parser.ParseIt.add_vfs_entry st.repl_fname code;
     let parse_result = parse_code None code in
     let log_syntax_issues err =
@@ -304,7 +345,7 @@ let run_full_buffer (st:repl_state)
         | ReloadDeps, d::_ ->
           run_qst (let! queries = reload_deps (!repl_stack) in
                    let! push_mod = push_decl FullCheck with_symbols write_full_buffer_fragment_progress d in
-                   return (queries @ push_mod, []))
+                   return (queries @ push_mod, [], st))
                   qid
 
         | _ ->
@@ -315,8 +356,10 @@ let run_full_buffer (st:repl_state)
             | Lax -> LaxCheck
             | _ -> FullCheck
           in
-          let queries, issues = 
-              run_qst (inspect_repl_stack (!repl_stack) decls push_kind with_symbols write_full_buffer_fragment_progress) qid
+          let queries, issues, st = 
+              run_qst (inspect_repl_stack
+                          (!repl_stack) st decls push_kind (request_type<>Cache)
+                          with_symbols write_full_buffer_fragment_progress) qid
           in
           if request_type <> Cache then log_syntax_issues err_opt;
           if Debug.any()
@@ -324,13 +367,13 @@ let run_full_buffer (st:repl_state)
             Format.print1 "Generating queries\n%s\n" 
                       (String.concat "\n" (List.map query_to_string queries))
           );
-          if request_type <> Cache then (queries, issues) else ([] , issues)
+          if request_type <> Cache then (queries, issues, st) else ([] , issues, st)
 
       )
         
       | ParseError err ->
         if request_type = Full then log_syntax_issues (Some err);
-        [], []
+        [], [], st
       | _ -> 
         failwith "Unexpected parse result"
     in
